src/impl/TLS13.Impl.Server.Types.fst
@@ -382,6 +382,25 @@ let server_local_event_input_ready
               (M.Certificate { M.chain = [cfg.CS.server_certificate_chain]; M.body = B.empty });
         })
      | None -> False)
+  | LocalSignCertificateVerify ->
+    Seq.equal payload B.empty /\
+    st.CS.cs_model.CS.model_control ==
+     CS.ControlHandshaking CS.HsServerEncryptedFlightSent /\
+    st.CS.cs_model.CS.model_config.CS.config_role == CS.ServerEndpoint /\
+    st.CS.cs_model.CS.model_handshake.CS.hs_certificate <> None /\
+    st.CS.cs_model.CS.model_handshake.CS.hs_certificate_verify == None /\
+    st.CS.cs_model.CS.model_handshake.CS.hs_buffers.CS.hb_certificate_verify_input == None /\
+    (match st.CS.cs_model.CS.model_config.CS.config_server,
+         st.CS.cs_model.CS.model_handshake.CS.hs_server_selection with
+     | Some cfg, Some selection ->
+     selection.CS.server_selected_signature_scheme ==
+         T.RsaPssRsaeSha256 /\
+     selection.CS.server_selected_credential ==
+         cfg.CS.server_credential_identity /\
+     CS.signature_scheme_offered
+         st.CS.cs_model.CS.model_config.CS.config_signature_schemes
+         T.RsaPssRsaeSha256
+     | _, _ -> False)
   | LocalSendEncryptedExtensions ->
     Seq.equal payload B.empty /\
     st.CS.cs_model.CS.model_control ==
